VisualProof/Rule/Executable.lean
@@ -6,3 +6,4 @@ import VisualProof.Rule.Executable.Vacuity
 import VisualProof.Rule.Executable.Presentation
 import VisualProof.Rule.Executable.Identification
 import VisualProof.Rule.Executable.WirePrimitive
+import VisualProof.Rule.Executable.Step
